slr-parsing/ambiguityScript.sml
@@ -1,0 +1,1458 @@
+open HolKernel boolLib bossLib Parse BasicProvers Defn
+
+open listTheory containerTheory pred_setTheory arithmeticTheory
+relationTheory markerTheory boolSimps optionTheory rich_listTheory
+pairTheory
+
+open regexpTheory grammarDefTheory boolLemmasTheory listLemmasTheory
+setLemmasTheory whileLemmasTheory parseTreeTheory followSetDefTheory
+parserDefTheory yaccDefTheory parseProp1DefTheory parseProp2DefTheory
+lrGrammarDefTheory validItemInvTheory macStepTheory complDefTheory
+
+
+fun MAGIC (asl, w) = ACCEPT_TAC (mk_thm(asl,w)) (asl,w) 
+
+val _ = Globals.linewidth := 60
+
+val _ = set_trace "Unicode" 1
+
+val isUnambiguous0 = 
+Define
+`isUnambiguous0 g = 
+     ∀sl.sl ∈ language g 
+            ==>
+     (∀dl dl'. (rderives g ⊢ dl ◁ [NTS (startSym g)] → sl ∧
+     rderives g ⊢ dl' ◁ [NTS (startSym g)] → sl) 
+        ⇒
+     (dl=dl'))`
+
+
+
+val listDiffPfxSame = store_thm
+("listDiffPfxSame" ,
+``∀l l'.¬(l=l') ==>
+(LENGTH l > LENGTH l' /\ ?sfx.l=l'++sfx) ∨
+(LENGTH l' > LENGTH l /\ ?sfx.l'=l++sfx) ∨
+(∃pfx h sfx h' sfx'.
+ (l=pfx++[h]++sfx) /\
+ (l'=pfx++[h']++sfx') /\ 
+ ¬(h=h'))``,
+Induct_on `l` THEN SRW_TAC [][] THEN
+Cases_on `l'` THEN FULL_SIMP_TAC (srw_ss()) []
+THENL[
+      METIS_TAC [APPEND_NIL,APPEND],
+
+      RES_TAC 
+      THENL[
+	    Cases_on `h=h'` THEN
+	    SRW_TAC [][] 
+            THENL[
+		  Cases_on `sfx` THEN FULL_SIMP_TAC (srw_ss()) [] THEN
+		  DISJ1_TAC THEN
+		  DECIDE_TAC,
+
+		  METIS_TAC [APPEND_NIL,APPEND]
+		  ],
+
+	    Cases_on `h=h'` THEN
+	    SRW_TAC [][] 
+	    THENL[
+		  DISJ2_TAC THEN
+		  FULL_SIMP_TAC (srw_ss()) [] THEN	    
+		  FULL_SIMP_TAC (arith_ss) [],
+		  
+		  METIS_TAC [APPEND_NIL,APPEND]
+		  ],
+
+	    Cases_on `h=h'` THEN
+	    SRW_TAC [][] 
+	    THENL[
+		  DISJ2_TAC THEN
+		  FULL_SIMP_TAC (srw_ss()) [] THEN	    
+		  FULL_SIMP_TAC (arith_ss) [],
+		  
+		  METIS_TAC [APPEND_NIL,APPEND]
+		  ] THEN
+	    METIS_TAC [APPEND_NIL,APPEND]
+      ]])
+
+
+val snoc_exists = store_thm
+("snoc_exists",
+``∀l.¬(l=[]) ==> ∃l'.((SNOC (LAST l) l') = l)``,
+HO_MATCH_MP_TAC SNOC_INDUCT THEN
+SRW_TAC [][] THEN
+Cases_on `l=[]`THEN FULL_SIMP_TAC (srw_ss())[]THEN
+SRW_TAC [][] 
+THENL[
+      Q.EXISTS_TAC `[]` THEN
+      SRW_TAC [][SNOC],
+      FULL_SIMP_TAC (srw_ss()) [SNOC_APPEND] THEN	    
+      Q.EXISTS_TAC `l` THEN
+      SRW_TAC [][] THEN	    
+      METIS_TAC [last_append,NOT_CONS_NIL,APPEND,LAST_CONS]
+      ])
+
+val listDiffSfxSame = store_thm
+("listDiffSfxSame" ,
+``∀l l'.¬(l=l') ==>
+(LENGTH l > LENGTH l' /\ ?pfx.l=pfx++l') ∨
+(LENGTH l' > LENGTH l /\ ?pfx.l'=pfx++l) ∨
+(∃pfx h pfx' h' sfx.
+ (l=pfx++[h]++sfx) /\
+ (l'=pfx'++[h']++sfx) /\ 
+ ¬(h=h'))``,
+HO_MATCH_MP_TAC SNOC_INDUCT THEN
+SRW_TAC [] [] 
+THENL[
+      Cases_on `l'` THEN FULL_SIMP_TAC (srw_ss()) [],
+
+ 
+      Cases_on `l'=[]` THEN FULL_SIMP_TAC (srw_ss()) [] 
+      THENL[
+	    FULL_SIMP_TAC (srw_ss()) [SNOC_APPEND] THEN
+	    DECIDE_TAC,
+
+	    `∃l''. l'=SNOC (LAST l') l''` 
+		by METIS_TAC [snoc_exists] THEN
+	    FULL_SIMP_TAC (srw_ss()) []  THEN
+	    SRW_TAC [][] THEN
+	    FULL_SIMP_TAC (srw_ss()) [SNOC_APPEND] THEN
+	    Q.ABBREV_TAC `x'=LAST l'` THEN
+	    FULL_SIMP_TAC (srw_ss()) [] THEN
+	    Cases_on `l=l''` THEN
+	    SRW_TAC [][] THEN
+	    FULL_SIMP_TAC (srw_ss()) [] THEN
+	    FULL_SIMP_TAC (arith_ss) []
+	    THENL[
+		  METIS_TAC [APPEND_NIL],
+
+		  RES_TAC THEN
+		  SRW_TAC [][] THEN
+		  FULL_SIMP_TAC (srw_ss()) [] THEN
+		  FULL_SIMP_TAC (arith_ss) [] 
+		  THENL[
+			Cases_on `x=x'` THEN
+			SRW_TAC [][] THEN
+			METIS_TAC [APPEND_NIL],
+
+			Cases_on `x=x'` THEN
+			SRW_TAC [][] THEN
+			METIS_TAC [APPEND_NIL],
+
+			Cases_on `x=x'` THEN
+			SRW_TAC [][] THEN
+			FULL_SIMP_TAC (srw_ss()) [] THEN
+			METIS_TAC [APPEND_NIL,APPEND_ASSOC]
+			]]]])
+
+
+val memLast = store_thm 
+("memLast",
+``∀l.¬(l=[]) ==> MEM (LAST l) l``,
+Induct_on `l` THEN SRW_TAC [][] THEN
+Cases_on `l` THEN FULL_SIMP_TAC (srw_ss()) [])
+
+
+
+val ntList = store_thm
+("ntList",
+``!s1 s2 n n' s1' s2'.
+(s1++[NTS n]++s2=s1'++[NTS n']++s2') ==>
+EVERY isTmnlSym (s2++s2') ==>
+(s1=s1') /\ (n=n') /\ (s2=s2')``,
+SRW_TAC [][] THEN
+`(s1' = s1++[NTS n]) ∨
+         (∃pfx sfx.
+            (s1++[NTS n] = s1' ++ [NTS n'] ++ pfx) ∧
+            (s2' = pfx ++ sfx)) ∨
+         ∃pfx sfx. (s1' = pfx ++ sfx) ∧ (s1++[NTS n] = pfx)`
+    by METIS_TAC [listCompLens,APPEND_ASSOC] THEN
+SRW_TAC [][] THEN
+FULL_SIMP_TAC (srw_ss()) []
+THENL[
+      `s2=[NTS n']++s2'` by METIS_TAC [APPEND_ASSOC,APPEND_11] THEN
+      FULL_SIMP_TAC (srw_ss()) [isTmnlSym_def],
+
+      Cases_on `pfx=[]`  THEN
+      SRW_TAC [][] THEN
+      FULL_SIMP_TAC (srw_ss()) [] 
+      THENL[
+	    METIS_TAC [lastElemEq,APPEND_11],
+	    `LAST [NTS n] = LAST pfx`
+		by METIS_TAC [last_append,APPEND_ASSOC,MEM,MEM_APPEND] THEN
+	    FULL_SIMP_TAC (srw_ss()) [] THEN
+	    `EVERY isTmnlSym (FRONT pfx ++ [NTS n])` by METIS_TAC [APPEND_FRONT_LAST] THEN
+	    FULL_SIMP_TAC (srw_ss()) [isTmnlSym_def]
+	    ],
+
+      `s2=sfx++[NTS n']++s2'` by METIS_TAC [APPEND_ASSOC,APPEND_11] THEN
+      SRW_TAC [][] THEN
+      FULL_SIMP_TAC (srw_ss()) [isTmnlSym_def],
+
+      `s2=[NTS n']++s2'` by METIS_TAC [APPEND_ASSOC,APPEND_11] THEN
+      SRW_TAC [][] THEN
+      FULL_SIMP_TAC (srw_ss()) [isTmnlSym_def],
+
+      Cases_on `pfx=[]`  THEN
+      SRW_TAC [][] THEN
+      FULL_SIMP_TAC (srw_ss()) [] 
+      THENL[
+	    METIS_TAC [lastElemEq,APPEND_11,symbol_11],
+	    `LAST [NTS n] = LAST pfx`
+		by METIS_TAC [last_append,APPEND_ASSOC,MEM,MEM_APPEND] THEN
+	    FULL_SIMP_TAC (srw_ss()) [] THEN
+	    `EVERY isTmnlSym (FRONT pfx ++ [NTS n])` by METIS_TAC [APPEND_FRONT_LAST] THEN
+	    FULL_SIMP_TAC (srw_ss()) [isTmnlSym_def]
+	    ],
+
+      `s2=sfx++[NTS n']++s2'` by METIS_TAC [APPEND_ASSOC,APPEND_11] THEN
+      SRW_TAC [][] THEN
+      FULL_SIMP_TAC (srw_ss()) [isTmnlSym_def],      
+
+      `s2=[NTS n']++s2'` by METIS_TAC [APPEND_ASSOC,APPEND_11] THEN
+      SRW_TAC [][] THEN
+      FULL_SIMP_TAC (srw_ss()) [isTmnlSym_def],
+
+      
+      Cases_on `pfx=[]`  THEN
+      SRW_TAC [][] THEN
+      FULL_SIMP_TAC (srw_ss()) []  THEN
+      `LAST [NTS n] = LAST pfx`
+	  by METIS_TAC [last_append,APPEND_ASSOC,MEM,MEM_APPEND] THEN
+      FULL_SIMP_TAC (srw_ss()) [] THEN
+      `EVERY isTmnlSym (FRONT pfx ++ [NTS n])` by METIS_TAC [APPEND_FRONT_LAST] THEN
+      FULL_SIMP_TAC (srw_ss()) [isTmnlSym_def],
+
+      `s2=sfx++[NTS n']++s2'` by METIS_TAC [APPEND_ASSOC,APPEND_11] THEN
+      SRW_TAC [][] THEN
+      FULL_SIMP_TAC (srw_ss()) [isTmnlSym_def]
+      ])
+
+
+val rtc2listRd = store_thm 
+("rtc2listRd",
+``!pfx sfx h h'.
+rtc2list R (pfx++[h]++[h']++sfx) ==>
+R h h'``,
+Induct_on `pfx` THEN SRW_TAC [][] THEN
+METIS_TAC [rtc2list_distrib_append_snd,MEM,MEM_APPEND,APPEND])
+
+val rtc2listSt = store_thm
+("rtc2listSt",
+``∀dl.(auggr g st eof = SOME ag) ==>
+ rsf ag (HD dl) ==>
+ rtc2list (rderives ag) dl ==>
+ ∀e.MEM e (TL dl) ==>  
+   ¬(e=[NTS (startSym ag)])``,
+
+Induct_on `dl` THEN SRW_TAC [][] THEN
+Cases_on `dl` THEN
+SRW_TAC [][] THEN
+FULL_SIMP_TAC (srw_ss()) [] THEN
+`rsf ag h'` by METIS_TAC [rsf_def,RTC_RULES_RIGHT1] THEN
+FULL_SIMP_TAC (srw_ss()) [] THEN
+SRW_TAC [][] THEN
+FULL_SIMP_TAC (srw_ss()) [rderives_def] THEN
+SRW_TAC [][] THEN
+FULL_SIMP_TAC (srw_ss()) [rsf_def] THEN
+SPOSE_NOT_THEN ASSUME_TAC THEN
+SRW_TAC [][] THEN
+Cases_on `lhs=startSym ag` 
+THENL[
+      SRW_TAC [][] THEN
+      `(s1=[]) /\ (s2=[])`by METIS_TAC [auggrRtcRderivesPfxSfxNil] THEN
+      SRW_TAC [][] THEN
+      FULL_SIMP_TAC (srw_ss()) [] THEN
+      METIS_TAC [auggrStNotInRhs,APPEND_NIL],
+
+      `?p.s2=p++[TS eof]` by METIS_TAC [lastEof] THEN
+      SRW_TAC [][] THEN
+      `LENGTH (s1 ++ rhs ++ p ++ [TS eof]) = 
+        LENGTH [NTS (startSym ag)]`
+      by METIS_TAC [APPEND_ASSOC] THEN
+      FULL_SIMP_TAC (srw_ss()) [] THEN
+      Cases_on `s1` THEN Cases_on `rhs` THEN
+      Cases_on `p` THEN FULL_SIMP_TAC (srw_ss()) []
+      ])
+      
+val slrConf1 = store_thm
+("slrConf1",
+``(slr ag = SOME m) ==>
+  (auggr g st eof = SOME ag) ==>
+  MEM (rule lhs rhs) (rules ag) ==>
+  MEM (rule lhs' rhs') (rules ag) ==>
+  rsf ag (s1 ++ [NTS lhs] ++ s) ==>
+  rsf ag (s1' ++ [NTS lhs'] ++ p ++ s) ==>
+  EVERY isTmnlSym (p ++ s) ==>
+ (s1 ++ rhs = s1' ++ rhs' ++ p) ==>
+ (s1 ++ [NTS lhs] = s1' ++ [NTS lhs'] ++ p)``,
+
+SRW_TAC [][] THEN
+`(s1 = s1'++rhs') ∧ (rhs = p) ∨
+ (∃px sx.
+     (s1 = s1' ++ rhs'++ px) ∧ (rhs = sx) ∧
+     (p = px ++ sx)) ∨
+ ∃px sx.
+ (s1'++rhs' = s1 ++ px) ∧ (p = sx) ∧ (rhs = px++sx)`
+    by METIS_TAC [twoListAppEq] THEN
+SRW_TAC [][]
+THENL[
+      FULL_SIMP_TAC (srw_ss()) [rsf_def] THEN
+      `?n.NRC (rderives ag) n 
+        [NTS (startSym ag)]
+	(s1' ++ rhs' ++ [NTS lhs] ++ s)`
+      by METIS_TAC [RTC_NRC] THEN
+      `?s.(trans ag (initItems ag (rules ag),s1' ++ rhs') =
+          SOME s) /\ MEM (item lhs ([],p)) s` 
+	  by METIS_TAC [lemma] THEN
+      `validItem ag (s1'++rhs') (item lhs' (rhs',[]))`
+      by (SRW_TAC [] [validItem_def] THEN
+	  Q.EXISTS_TAC `p++s` THEN
+	  SRW_TAC [][] THEN
+	  METIS_TAC [rderives_append,rdres1,EVERY_APPEND,APPEND_ASSOC]) THEN
+      `MEM (item lhs' (rhs',[])) s'` 
+	  by METIS_TAC [transImpValidItem] THEN
+      Cases_on `lhs=startSym ag` THEN
+      SRW_TAC [][]
+      THENL[
+	    `p=[NTS (startSym g);TS eof]` by METIS_TAC [auggrStartRule] THEN
+	    SRW_TAC [][] THEN
+	    `(s1'++rhs'=[]) /\ (s=[])`
+	    by METIS_TAC [auggrRtcRderivesPfxSfxNil] THEN
+	    SRW_TAC [][] THEN
+	    FULL_SIMP_TAC (srw_ss()) [isTmnlSym_def],
+	    
+	    `?h t.p++s=h::t` by METIS_TAC [list_nchotomy,MEM,MEM_APPEND,lastEof] THEN
+	    SRW_TAC [][] THEN
+	    `h IN (followSet ag (NTS lhs'))` by METIS_TAC [followSetMem, APPEND, APPEND_ASSOC, APPEND_NIL, rtcRdImpDg, isTmnlSym_def,EVERY_DEF,EVERY_APPEND] THEN
+	    Cases_on `p` THEN
+	    FULL_SIMP_TAC (srw_ss()) []
+	    THENL[
+		  SRW_TAC [][] THEN
+		  `h IN (followSet ag (NTS lhs))` by METIS_TAC [followSetMem, APPEND, APPEND_ASSOC, APPEND_NIL, rtcRdImpDg, isTmnlSym_def,EVERY_DEF,EVERY_APPEND] THEN
+		  `(item lhs' (rhs',[])=(item lhs ([],[])))` 
+		      by METIS_TAC [transImpValidItem,completeItem_def,
+				    itemLhs_def,slrCompItemsEq] THEN
+		  FULL_SIMP_TAC (srw_ss()) [],
+
+		  SRW_TAC [][] THEN
+		  METIS_TAC [slrNotValid,sgoto_exp]
+		  ]
+	    ],
+
+
+      FULL_SIMP_TAC (srw_ss()) [rsf_def] THEN
+      SRW_TAC [][] THEN
+      `?n.NRC (rderives ag) n [NTS (startSym ag)]
+            (s1' ++ rhs' ++ px ++ [NTS lhs] ++ s)`
+      by METIS_TAC [RTC_NRC] THEN
+      `?s.(trans ag (initItems ag (rules ag),s1' ++ rhs'++px) =
+          SOME s) /\ MEM (item lhs ([],rhs)) s` 
+	  by METIS_TAC [lemma] THEN      
+      `validItem ag (s1'++rhs') (item lhs' (rhs',[]))`
+      by (SRW_TAC [][validItem_def] THEN
+	  Q.EXISTS_TAC `px++rhs++s` THEN SRW_TAC [][] THEN
+	  METIS_TAC [rdres1,rderives_append,EVERY_APPEND,APPEND_ASSOC]) THEN
+      `?s''.(trans ag (initItems ag (rules ag),s1' ++ rhs') =
+	     SOME s'') /\ (trans ag (s'',px) = SOME s')` 
+	  by METIS_TAC [transAppend] THEN          
+      `MEM (item lhs' (rhs',[])) s''`
+      by METIS_TAC [transImpValidItem] THEN
+      Cases_on `lhs=startSym ag` THEN
+      SRW_TAC [][]
+      THENL[
+	    `rhs=[NTS (startSym g); TS eof]`
+		by METIS_TAC [auggrStartRule] THEN
+	    SRW_TAC [][] THEN
+	    `(s1'++rhs'++px=[]) /\ (s=[])`
+		by METIS_TAC [auggrRtcRderivesPfxSfxNil] THEN
+	    FULL_SIMP_TAC (srw_ss()) [] THEN
+	    SRW_TAC [][] THEN
+	    FULL_SIMP_TAC (srw_ss()) [isTmnlSym_def],
+
+	    `¬(s=[])` by METIS_TAC [lastEof,MEM,MEM_APPEND] THEN
+	    `¬(px++rhs++s = [])` by SRW_TAC [][] THEN
+	    Cases_on `px` THEN SRW_TAC [][]
+            THENL[
+		  FULL_SIMP_TAC (srw_ss()) [trans_def] THEN
+		  Cases_on `rhs` THEN FULL_SIMP_TAC (srw_ss()) [] THEN
+		  SRW_TAC [][] 
+		  THENL[
+			`h IN (followSet ag (NTS lhs'))` by METIS_TAC [followSetMem, APPEND, APPEND_ASSOC, APPEND_NIL, rtcRdImpDg, isTmnlSym_def,EVERY_DEF,EVERY_APPEND] THEN			
+			METIS_TAC [slrNotValid,sgoto_exp,EVERY_DEF],
+
+			Cases_on `s` THEN FULL_SIMP_TAC (srw_ss()) [] THEN
+			`h IN (followSet ag (NTS lhs'))` by METIS_TAC [followSetMem, APPEND, APPEND_ASSOC, APPEND_NIL, rtcRdImpDg, isTmnlSym_def,EVERY_DEF,EVERY_APPEND] THEN						
+			`h IN (followSet ag (NTS lhs))` by METIS_TAC [followSetMem, APPEND, APPEND_ASSOC, APPEND_NIL, rtcRdImpDg, isTmnlSym_def,EVERY_DEF,EVERY_APPEND] THEN						
+			`(item lhs' (rhs',[])=(item lhs ([],[])))` 
+			    by METIS_TAC [transImpValidItem,completeItem_def,
+					  itemLhs_def,slrCompItemsEq] THEN
+			FULL_SIMP_TAC (srw_ss()) [],
+			
+			`h IN (followSet ag (NTS lhs'))` by METIS_TAC [followSetMem, APPEND, APPEND_ASSOC, APPEND_NIL, rtcRdImpDg, isTmnlSym_def,EVERY_DEF,EVERY_APPEND] THEN						
+			METIS_TAC [slrNotValid,sgoto_exp,EVERY_DEF]
+			],		  
+		  
+		  FULL_SIMP_TAC (srw_ss()) [trans_def] THEN
+		  Cases_on `moveDot s'' h` THEN 
+		  FULL_SIMP_TAC (srw_ss()) [] THEN
+		  `∃l r1 r2.
+                     (h' = item l (r1 ++ [h],r2)) ∧
+                     MEM (item l (r1,h::r2)) s''`
+		      by METIS_TAC [mdMem,MEM] THEN
+		  `h IN (followSet ag (NTS lhs'))` by METIS_TAC [followSetMem, APPEND, APPEND_ASSOC, APPEND_NIL, rtcRdImpDg, isTmnlSym_def,EVERY_DEF,EVERY_APPEND] THEN						
+		  METIS_TAC [slrNotValid,sgoto_exp,EVERY_DEF]		  
+		  ]
+	    ],
+
+      
+      FULL_SIMP_TAC (srw_ss()) [rsf_def] THEN
+      SRW_TAC [][] THEN
+      `∃n.NRC (rderives ag) n [NTS (startSym ag)]
+            (s1 ++ [NTS lhs] ++ s)` 
+      by METIS_TAC [RTC_NRC] THEN
+      `∃s.(trans ag (initItems ag (rules ag),s1) = SOME s) /\
+          MEM (item lhs ([],px ++ p)) s`
+      by METIS_TAC [lemma] THEN
+      Cases_on `lhs=startSym ag`  THEN SRW_TAC [][]
+      THENL[
+	    `px++p=[NTS (startSym g);TS eof]`
+	    by METIS_TAC [auggrStartRule] THEN
+	    `(s1=[]) /\ (s=[])` by METIS_TAC [auggrRtcRderivesPfxSfxNil] THEN
+	    SRW_TAC [][] THEN
+	    FULL_SIMP_TAC (srw_ss()) [] THEN
+	    Cases_on `lhs'=startSym ag` THEN
+	    SRW_TAC [][]
+	    THENL[
+		  METIS_TAC [auggrRtcRderivesPfxSfxNil,APPEND_NIL],
+
+		  FULL_SIMP_TAC (srw_ss()) [trans_def] THEN
+		  Cases_on `s1'` THEN
+		  Cases_on `rhs'` THEN
+		  Cases_on `p` THEN
+		  SRW_TAC [][] THEN
+		  FULL_SIMP_TAC (srw_ss()) [isTmnlSym_def]
+                  THENL[
+			SRW_TAC [][] THEN
+			METIS_TAC [APPEND,APPEND_NIL,auggrEofInRhs,MEM,MEM_APPEND],
+
+			SRW_TAC [][] THEN
+			Cases_on `t` THEN FULL_SIMP_TAC (srw_ss()) [] THEN
+			SRW_TAC [][] THEN
+			`MEM (item lhs' ([],[NTS (startSym g)]))
+		          (initItems ag (rules ag))`
+			by METIS_TAC [initItemsHdNt,APPEND] THEN
+			`TS eof ∈ (followSet ag (NTS lhs'))` by METIS_TAC [followSetMem, APPEND, APPEND_ASSOC, APPEND_NIL, rtcRdImpDg, isTmnlSym_def,EVERY_DEF,EVERY_APPEND] THEN						
+			`∃s.(trans ag (initItems ag (rules ag),[NTS (startSym g)])
+			   = SOME s) /\ 
+                          MEM (item lhs' ([NTS (startSym g)],[])) s /\
+                          MEM (item (startSym ag) ([NTS (startSym g)],[TS eof])) s` 
+			    by (SRW_TAC [][trans_def] THEN
+			Cases_on `moveDot (initItems ag (rules ag)) (NTS (startSym g))` THEN
+			SRW_TAC [][] THEN
+			METIS_TAC [mdMemExists,APPEND,APPEND_NIL,MEM,iclosure_mem]) THEN
+			METIS_TAC [isTmnlSym_def,sgoto_exp,slrNotValid],
+
+			SRW_TAC [][] THEN
+			`[NTS (startSym g); TS eof; NTS lhs']=
+           		  [NTS (startSym g); TS eof]++ [NTS lhs']`
+			    by SRW_TAC [][] THEN
+			METIS_TAC [APPEND_NIL,lastEof,MEM,MEM_APPEND],
+
+
+			Cases_on `t` THEN FULL_SIMP_TAC (srw_ss()) [] THEN
+			SRW_TAC [][] THEN
+			`[NTS (startSym g); NTS lhs'; TS eof]=
+                           [NTS (startSym g)]++ [NTS lhs']++[TS eof]`
+			    by SRW_TAC [][] THEN
+			`∃s.(trans ag (initItems ag (rules ag),[NTS (startSym g)]) = SOME s)
+                          /\ MEM (item lhs' ([],[])) s`
+			    by METIS_TAC [lemma,RTC_NRC] THEN
+			`validItem ag [NTS (startSym g)] (item (startSym ag) ([NTS (startSym g)], [TS eof]))`
+			    by (SRW_TAC [] [validItem_def] THEN
+				MAP_EVERY Q.EXISTS_TAC [`[]`,`[]`] THEN
+				SRW_TAC [][] THEN
+				METIS_TAC [rdres1]) THEN
+			`TS eof ∈ (followSet ag (NTS lhs'))` by METIS_TAC [followSetMem, APPEND, APPEND_ASSOC, APPEND_NIL, rtcRdImpDg, isTmnlSym_def,EVERY_DEF,EVERY_APPEND] THEN						
+			METIS_TAC [slrNotValid,isTmnlSym_def,APPEND,sgoto_exp,transImpValidItem],
+
+			Cases_on `t` THEN FULL_SIMP_TAC (srw_ss()) [] THEN
+			SRW_TAC [][]THEN
+			METIS_TAC [auggrEofInRhs,APPEND_NIL],
+
+			Cases_on `t` THEN FULL_SIMP_TAC (srw_ss()) []
+			]
+		  ],
+
+	    `¬(s=[])` by METIS_TAC [lastEof,MEM,MEM_APPEND] THEN
+	    Cases_on `s` THEN SRW_TAC [][] THEN
+	    `h ∈ (followSet ag (NTS lhs))` by METIS_TAC [followSetMem, APPEND, APPEND_ASSOC, APPEND_NIL, rtcRdImpDg, isTmnlSym_def,EVERY_DEF,EVERY_APPEND] THEN						
+	    IMP_RES_TAC twoListAppEq THEN
+	    SRW_TAC [][]
+	    THENL[
+		  `validItem ag s1 (item lhs' ([],px))`
+		      by (SRW_TAC [] [validItem_def] THEN
+			  Q.EXISTS_TAC `p++h::t` THEN
+			  SRW_TAC [][] THEN
+			  METIS_TAC [rdres1,EVERY_APPEND,
+				     rderives_append,APPEND,
+				     EVERY_DEF,APPEND_ASSOC]) THEN
+		  `MEM (item lhs' ([],px)) s'` by METIS_TAC [transImpValidItem] THEN
+		  Cases_on `px` THEN
+		  Cases_on `p` THEN
+		  SRW_TAC [][] THEN
+		  FULL_SIMP_TAC (srw_ss()) []
+		  THENL[
+
+			`h ∈ (followSet ag (NTS lhs'))` by METIS_TAC [followSetMem, APPEND, APPEND_ASSOC, APPEND_NIL, rtcRdImpDg, isTmnlSym_def,EVERY_DEF,EVERY_APPEND] THEN									
+			METIS_TAC [transImpValidItem,completeItem_def,
+				   itemLhs_def,slrCompItemsEq],
+
+			`h' ∈ (followSet ag (NTS lhs'))` by METIS_TAC [followSetMem, APPEND, APPEND_ASSOC, APPEND_NIL, rtcRdImpDg, isTmnlSym_def,EVERY_DEF,EVERY_APPEND] THEN
+			METIS_TAC [slrNotValid,sgoto_exp],
+
+			`h ∈ (followSet ag (NTS lhs'))` by METIS_TAC [followSetMem, APPEND, APPEND_ASSOC, APPEND_NIL, rtcRdImpDg, isTmnlSym_def,EVERY_DEF,EVERY_APPEND] THEN									
+			`∃s''. trans ag (s',h'::t') = SOME s''`
+			    by METIS_TAC [ruleRhsExistsImpTrans] THEN
+			`validItem ag (s1++h'::t') (item lhs' (h'::t',[]))`
+			    by (SRW_TAC [] [validItem_def] THEN
+				Q.EXISTS_TAC `h::t` THEN
+				SRW_TAC [][] THEN
+				METIS_TAC [rdres1,EVERY_APPEND,
+					   rderives_append,APPEND,
+					   EVERY_DEF,APPEND_ASSOC]) THEN
+			`validItem ag (s1++h'::t') (item lhs (h'::t',[]))`
+			    by (SRW_TAC [] [validItem_def] THEN
+				Q.EXISTS_TAC `h::t` THEN
+				SRW_TAC [][] THEN
+				METIS_TAC [rdres1,EVERY_APPEND,
+					   rderives_append,APPEND,
+					   EVERY_DEF,APPEND_ASSOC]) THEN
+			`trans ag (initItems ag (rules ag),s1++h'::t') = SOME s''`
+			    by METIS_TAC [transSeq,initItems_def] THEN
+			METIS_TAC [transImpValidItem,completeItem_def,
+				   itemLhs_def,slrCompItemsEq],
+
+			`∃s''. trans ag (s',h'::t') = SOME s''`
+			    by METIS_TAC [ruleRhsExistsImpTrans] THEN
+			`validItem ag (s1++h'::t') (item lhs' (h'::t',[]))`
+			    by (SRW_TAC [] [validItem_def] THEN
+				Q.EXISTS_TAC `h''::t''++h::t` THEN
+				SRW_TAC [][] THEN
+				METIS_TAC [rdres1,EVERY_APPEND,
+					   rderives_append,APPEND,
+					   EVERY_DEF,APPEND_ASSOC]) THEN
+			`validItem ag (s1++h'::t') (item lhs (h'::t',h''::t''))`
+			    by (SRW_TAC [] [validItem_def] THEN
+				Q.EXISTS_TAC `h::t` THEN
+				SRW_TAC [][] THEN
+				`(s1 ++ h'::t' ++ h''::t'' ++ h::t) 
+                                  = s1 ++ (h'::(t' ++ h''::t'')) ++ h::t`
+				    by METIS_TAC [APPEND_ASSOC,APPEND] THEN
+				METIS_TAC [rdres1,rderives_append,EVERY_DEF]) THEN
+			`trans ag (initItems ag (rules ag),s1++h'::t') = SOME s''`
+			    by METIS_TAC [transSeq,initItems_def] THEN
+			`h'' ∈ (followSet ag (NTS lhs'))` by METIS_TAC [followSetMem, APPEND, APPEND_ASSOC, APPEND_NIL, rtcRdImpDg, isTmnlSym_def,EVERY_DEF,EVERY_APPEND] THEN									
+			METIS_TAC [slrNotValid,sgoto_exp, transImpValidItem]
+			],
+
+
+		  Cases_on `p` THEN SRW_TAC [][] THEN
+		  Cases_on `s1''` THEN SRW_TAC [][] THEN
+		  FULL_SIMP_TAC (srw_ss()) []
+		  THENL[
+			`∃s.(trans ag (initItems ag (rules ag),s1) = SOME s)
+                          /\ MEM (item lhs ([],rhs')) s`
+			by METIS_TAC [lemma] THEN
+			`MEM (item lhs' ([],rhs')) s`
+			    by METIS_TAC [lemma,transOutEq,RTC_NRC] THEN
+			IMP_RES_TAC ruleRhsExistsImpTrans THEN
+			`h ∈ (followSet ag (NTS lhs'))` by METIS_TAC [followSetMem, APPEND, APPEND_ASSOC, APPEND_NIL, rtcRdImpDg, isTmnlSym_def,EVERY_DEF,EVERY_APPEND] THEN
+			`validItem ag (s1++rhs') (item lhs (rhs',[]))`
+			    by (SRW_TAC [][validItem_def] THEN
+				Q.EXISTS_TAC `h::t` THEN
+				SRW_TAC [][] THEN
+				METIS_TAC [rdres1,EVERY_DEF,rderives_append]) THEN
+			`validItem ag (s1++rhs') (item lhs' (rhs',[]))`
+			    by (SRW_TAC [][validItem_def] THEN
+				Q.EXISTS_TAC `h::t` THEN
+				SRW_TAC [][] THEN
+				METIS_TAC [rdres1,EVERY_DEF,rderives_append]) THEN
+			`(∃s'. (trans ag (s,rhs') = SOME s')) /\ ∃s''. (trans ag (s',rhs') = SOME s'')`
+			    by METIS_TAC [] THEN
+			`s''=s'''` by METIS_TAC [transOutEq] THEN
+			SRW_TAC [][] THEN
+			`trans ag (initItems ag (rules ag),s1++rhs') = SOME s''` by METIS_TAC [transSeq,initItems_def] THEN
+			METIS_TAC [slrCompItemsEq,itemLhs_def,completeItem_def,transImpValidItem],
+
+
+			`∃s.(trans ag (initItems ag (rules ag),s1) = SOME s)
+                          /\ MEM (item lhs ([],h'::(t'++rhs'))) s`
+			by METIS_TAC [lemma] THEN
+			`validItem ag (s1++h'::t'++rhs') (item lhs' (rhs',[]))`
+			    by (SRW_TAC [][validItem_def] THEN
+				Q.EXISTS_TAC `h::t` THEN
+				SRW_TAC [][] THEN
+				METIS_TAC [rdres1,rderives_append,EVERY_DEF,APPEND_ASSOC]) THEN
+			`validItem ag (s1++h'::t'++rhs') (item lhs (h'::(t'++rhs'),[]))`
+			    by (SRW_TAC [][validItem_def] THEN
+			        Q.EXISTS_TAC `s1` THEN
+				Q.EXISTS_TAC `h::t` THEN
+				SRW_TAC [][] 
+				THENL[
+				      METIS_TAC [rdres1,rderives_append,EVERY_DEF,APPEND_ASSOC],
+				      METIS_TAC [APPEND,APPEND_ASSOC]]) THEN
+			`∃s'. trans ag (s,h'::(t' ++ rhs')) = SOME s'`
+			    by METIS_TAC [ruleRhsExistsImpTrans] THEN			
+			`trans ag (initItems ag (rules ag),s1++h'::(t' ++ rhs')) = SOME s''`
+			    by METIS_TAC [transSeq,initItems_def] THEN
+			`h ∈ (followSet ag (NTS lhs'))` 
+			    by METIS_TAC [followSetMem, APPEND, APPEND_ASSOC,rtcRdImpDg, 
+					  isTmnlSym_def,EVERY_DEF,EVERY_APPEND] THEN
+			`h'::(t'++rhs') = h'::t'++rhs'`
+			    by METIS_TAC [APPEND,APPEND_ASSOC] THEN
+			`MEM (item lhs (h'::(t' ++ rhs'),[])) s''`
+			    by METIS_TAC [transImpValidItem,APPEND_ASSOC] THEN
+			`MEM (item lhs' (rhs',[])) s''` 
+			    by METIS_TAC [transImpValidItem,APPEND_ASSOC]  THEN
+			`(item lhs' (rhs',[]) = item lhs (h'::(t' ++ rhs'),[]))`
+			    by METIS_TAC [slrCompItemsEq,itemLhs_def,completeItem_def,transImpValidItem] THEN
+			FULL_SIMP_TAC (srw_ss()) [] THEN
+			METIS_TAC [APPEND_11,APPEND,APPEND_ASSOC],
+
+			`∃s.(trans ag (initItems ag (rules ag),s1) = SOME s)
+                          /\ MEM (item lhs ([],rhs'++h'::t')) s`
+			by METIS_TAC [lemma] THEN
+			`∃s'. trans ag (s,rhs' ++ h'::t') = SOME s'`
+			    by METIS_TAC [ruleRhsExistsImpTrans] THEN
+			`trans ag (initItems ag (rules ag),s1++rhs'++h'::t') = SOME s''`
+			by METIS_TAC [transSeq,initItems_def,APPEND_ASSOC] THEN
+			`?s'''.trans ag (initItems ag (rules ag),s1++rhs') = SOME s'''`
+			by METIS_TAC [transOverAppend] THEN
+			`validItem ag (s1++rhs') (item lhs (rhs',h'::t'))`
+			by (SRW_TAC [] [validItem_def] THEN
+			    Q.EXISTS_TAC `h::t` THEN
+			    SRW_TAC [] [] THEN
+			    METIS_TAC [rdres1,rderives_append,EVERY_DEF,APPEND_ASSOC]) THEN
+			`validItem ag (s1++rhs') (item lhs' (rhs',[]))`
+			    by (SRW_TAC [] [validItem_def] THEN
+			    Q.EXISTS_TAC `h'::t'++h::t` THEN
+			    SRW_TAC [] [] THEN
+			    METIS_TAC [rdres1,rderives_append,EVERY_DEF,APPEND_ASSOC,EVERY_APPEND]) THEN
+			`h' ∈ (followSet ag (NTS lhs'))` 
+			    by METIS_TAC [followSetMem, APPEND, APPEND_ASSOC,rtcRdImpDg, 
+					  isTmnlSym_def,EVERY_DEF,EVERY_APPEND] THEN			
+			METIS_TAC [slrNotValid,sgoto_exp,transImpValidItem],
+
+
+			`∃s.(trans ag (initItems ag (rules ag),s1++h''::t'') = SOME s)
+                          /\ MEM (item lhs' ([],rhs')) s`
+			by METIS_TAC [lemma,RTC_NRC,APPEND_ASSOC] THEN
+			`∃s'. trans ag (s,rhs') = SOME s'` 
+			    by METIS_TAC [ruleRhsExistsImpTrans] THEN
+			`trans ag (initItems ag (rules ag),s1 ++ h''::t''++rhs') 
+		          = SOME s''` by METIS_TAC [transSeq,initItems_def] THEN
+			`validItem ag (s1 ++ h''::t'' ++ rhs') (item lhs' (rhs',[]))`
+			by (SRW_TAC [] [validItem_def] THEN
+			    Q.EXISTS_TAC `h'::t'++h::t` THEN
+			    SRW_TAC [][] THEN
+			    `(s1 ++ h''::t'' ++ rhs' ++ h'::t' ++ h::t) =
+              			(s1 ++ h''::t'') ++ rhs' ++ (h'::t' ++ h::t)`
+				by METIS_TAC [APPEND_ASSOC] THEN
+			    `EVERY isTmnlSym (h'::t' ++ h::t)` by FULL_SIMP_TAC (srw_ss()) [] THEN
+			    METIS_TAC [rdres1,rderives_append,APPEND_ASSOC]) THEN
+			`validItem ag (s1 ++ h''::t'' ++ rhs') (item lhs ((h''::t'' ++ rhs'), h'::t'))`
+			by (SRW_TAC [] [validItem_def] THEN
+			    Q.EXISTS_TAC `h::t` THEN
+			    SRW_TAC [][] THEN
+			    `(s1 ++ h''::t'' ++ rhs' ++ h'::t' ++ h::t)=
+                               (s1 ++ (h''::t'' ++ rhs' ++ h'::t') ++ h::t)`
+				by METIS_TAC [APPEND_ASSOC] THEN
+			    `h''::(t''++rhs'++h'::t') = h''::t''++rhs'++h'::t'`
+				by SRW_TAC [][] THEN
+			    METIS_TAC [rdres1,EVERY_DEF,rderives_append]) THEN
+			`h' ∈ (followSet ag (NTS lhs'))` 
+			    by METIS_TAC [followSetMem, APPEND, APPEND_ASSOC,rtcRdImpDg, 
+					  isTmnlSym_def,EVERY_DEF,EVERY_APPEND] THEN			
+			METIS_TAC [slrNotValid,sgoto_exp,transImpValidItem]
+			],
+
+		  Cases_on `s1''` THEN
+		  SRW_TAC [][]
+		  THENL[
+			FULL_SIMP_TAC (srw_ss()) []THEN
+			Cases_on `px` THEN
+			Cases_on `p` THEN
+			SRW_TAC [][] THEN
+			FULL_SIMP_TAC (srw_ss()) []
+			THENL[
+			      `MEM (item lhs' ([],[])) s'`
+			      by METIS_TAC [lemma,RTC_NRC,transOutEq] THEN
+			      `h ∈ (followSet ag (NTS lhs'))` 
+				  by METIS_TAC [followSetMem, APPEND, APPEND_ASSOC,rtcRdImpDg, 
+					  isTmnlSym_def,EVERY_DEF,EVERY_APPEND] THEN						      
+			      METIS_TAC [slrCompItemsEq,itemLhs_def,completeItem_def],
+
+			      `MEM (item lhs' ([],[])) s'`
+			      by METIS_TAC [lemma,RTC_NRC,transOutEq,APPEND_ASSOC] THEN
+			      `h' ∈ (followSet ag (NTS lhs'))` 
+				  by METIS_TAC [followSetMem, APPEND, APPEND_ASSOC,rtcRdImpDg, 
+					  isTmnlSym_def,EVERY_DEF,EVERY_APPEND] THEN						      
+			      METIS_TAC [slrNotValid,sgoto_exp],
+
+			      IMP_RES_TAC ruleRhsExistsImpTrans THEN
+			      `∃s''. trans ag (s',h'::t') = SOME s''`
+			      by METIS_TAC [] THEN
+			      `trans ag (initItems ag (rules ag),s1'++h'::t') = SOME s''`
+			      by METIS_TAC [transSeq,initItems_def] THEN
+			      `validItem ag (s1'++h'::t') (item lhs (h'::t',[]))`
+			      by (SRW_TAC [][validItem_def] THEN
+				  Q.EXISTS_TAC `h::t` THEN
+				  SRW_TAC [][] THEN
+				  METIS_TAC [rdres1,rderives_append,EVERY_DEF]) THEN
+			      `validItem ag (s1'++h'::t') (item lhs' (h'::t',[]))`
+			      by (SRW_TAC [][validItem_def] THEN
+				  Q.EXISTS_TAC `h::t` THEN
+				  SRW_TAC [][] THEN
+				  METIS_TAC [rdres1,rderives_append,EVERY_DEF]) THEN
+			      `h ∈ (followSet ag (NTS lhs'))` 
+				  by METIS_TAC [followSetMem, APPEND, APPEND_ASSOC,rtcRdImpDg, 
+					  isTmnlSym_def,EVERY_DEF,EVERY_APPEND] THEN		
+			      METIS_TAC [transImpValidItem,slrCompItemsEq,itemLhs_def,completeItem_def],
+
+
+			      `∃s''.trans ag (s',h'::(t' ++ h''::t'')) = SOME s''`
+			      by METIS_TAC [ruleRhsExistsImpTrans] THEN
+			      `?s.trans ag (s',h'::t') = SOME s`
+			      by METIS_TAC [APPEND,APPEND_ASSOC,transOverAppend] THEN
+			      `trans ag (initItems ag (rules ag),s1'++h'::t') = SOME s`
+				  by METIS_TAC [transSeq,initItems_def] THEN
+			      `validItem ag (s1'++h'::t') (item lhs (h'::t',h''::t''))`
+			      by (SRW_TAC [][validItem_def] THEN
+				  Q.EXISTS_TAC `h::t` THEN
+				  `(h'::(t' ++ h''::t'')=h'::t' ++ h''::t'')`
+				      by METIS_TAC [APPEND_ASSOC,APPEND] THEN			
+				  SRW_TAC [][]  THEN
+				  METIS_TAC [rdres1,rderives_append,EVERY_DEF,APPEND_ASSOC]) THEN
+			      `validItem ag (s1'++h'::t') (item lhs' (h'::t',[]))`
+			      by (SRW_TAC [][validItem_def] THEN
+				  Q.EXISTS_TAC `h''::t''++h::t` THEN
+				  SRW_TAC [][] THEN
+				  `EVERY isTmnlSym (h''::t'' ++ h::t)` by FULL_SIMP_TAC (srw_ss()) [] THEN
+				  METIS_TAC [rdres1,rderives_append,APPEND_ASSOC]) THEN
+			      `h'' ∈ (followSet ag (NTS lhs'))` 
+				  by METIS_TAC [followSetMem, APPEND, APPEND_ASSOC,rtcRdImpDg, 
+					  isTmnlSym_def,EVERY_DEF,EVERY_APPEND] THEN
+			      METIS_TAC [slrNotValid,sgoto_exp,transImpValidItem]
+			      ],
+			
+			`validItem ag (s1'++h'::t'++px) 
+		           (item lhs (px,p))`
+			by (SRW_TAC [] [validItem_def] THEN
+			    Q.EXISTS_TAC `h::t` THEN
+			    SRW_TAC [][] THEN
+			    METIS_TAC [rderives_append,rdres1,
+				       EVERY_DEF,APPEND_ASSOC]) THEN
+			`validItem ag (s1'++h'::t'++px) 
+			   (item lhs' (h'::t'++px,[])) `
+			by (SRW_TAC [] [validItem_def] THEN
+			    Q.EXISTS_TAC `p++h::t` THEN
+			    `h'::t'++px=h'::(t'++px)`
+				by SRW_TAC [][] THEN
+			    METIS_TAC [rdres1,rderives_append,
+				       EVERY_DEF,APPEND_ASSOC,
+				       EVERY_APPEND]) THEN
+			`∃s''. trans ag (s',px ++ p) = SOME s''` 
+			    by METIS_TAC[ruleRhsExistsImpTrans] THEN
+			`trans ag (initItems ag (rules ag),(s1' ++ h'::t') ++ (px++p)) = SOME s''`
+			by METIS_TAC [transSeq,initItems_def] THEN
+			`?sx.trans ag (initItems ag (rules ag),s1' ++ h'::t' ++ px ) =
+		         SOME sx`
+			by METIS_TAC [transOverAppend,APPEND_ASSOC] THEN
+			Cases_on `p` THEN SRW_TAC [][] THEN
+			FULL_SIMP_TAC (srw_ss()) []
+			THENL[
+			      `h ∈ (followSet ag (NTS lhs'))` 
+				  by METIS_TAC [followSetMem, APPEND, APPEND_ASSOC,rtcRdImpDg, 
+					  isTmnlSym_def,EVERY_DEF,EVERY_APPEND] THEN			      
+			      `(item lhs' (h'::(t' ++ px),[])=(item lhs (px,[])))` 
+				  by METIS_TAC [slrCompItemsEq,itemLhs_def,completeItem_def,transImpValidItem] THEN
+			      FULL_SIMP_TAC (srw_ss()) [] THEN
+			      SRW_TAC [][] THEN
+			      METIS_TAC [APPEND_11,APPEND_ASSOC,NOT_CONS_NIL,APPEND],
+
+			      `h'' ∈ (followSet ag (NTS lhs'))` 
+				  by METIS_TAC [followSetMem, APPEND, APPEND_ASSOC,rtcRdImpDg, 
+					  isTmnlSym_def,EVERY_DEF,EVERY_APPEND] THEN			      
+			      METIS_TAC [transImpValidItem,slrNotValid,sgoto_exp]			      
+			      ]
+			]
+		  ]]])
+
+
+
+val slrConf = store_thm	
+("slrConf",
+``(slr ag = SOME m) ==>
+  (auggr g st eof = SOME ag)==>
+  MEM (rule lhs rhs) (rules ag) ==>
+  MEM (rule lhs' rhs') (rules ag) ==>
+  rsf ag (s1 ++ [NTS lhs] ++ s2) ==>
+  rsf ag (s1' ++ [NTS lhs'] ++ s2') ==>
+  EVERY isTmnlSym (s2++s2') ==>
+  (s1 ++ rhs ++ s2 = s1' ++ rhs' ++ s2') ==>
+  (s1 ++ [NTS lhs] ++ s2 = s1' ++ [NTS lhs'] ++ s2')``,
+
+SRW_TAC [][] THEN
+`(s1 ++ rhs) ++ s2 = (s1' ++ rhs') ++ s2'`
+    by METIS_TAC [APPEND_ASSOC] THEN
+`(s1++rhs = s1'++rhs') ∧ (s2 = s2') ∨
+       (∃p s.
+          (s1++rhs = (s1'++rhs') ++ p) ∧ (s2 = s) ∧
+          (s2' = p ++ s)) ∨
+       ∃p s.
+         (s1'++rhs' = (s1++rhs) ++ p) ∧ (s2' = s) ∧ (s2 = p ++ s)`
+    by METIS_TAC [twoListAppEq] THEN
+SRW_TAC [][]
+THENL[
+      `(s1 = s1') ∧ (rhs = rhs') ∨
+       (∃p s.
+          (s1 = s1' ++ p) ∧ (rhs = s) ∧
+          (rhs' = p ++ s)) ∨
+       ∃p s.
+         (s1' = s1 ++ p) ∧ (rhs' = s) ∧ (rhs = p++s)`
+      by METIS_TAC [twoListAppEq] THEN
+      SRW_TAC [][]
+      THENL[
+	    FULL_SIMP_TAC (srw_ss()) [rsf_def] THEN
+	    `?n.NRC (rderives ag) n 
+              [NTS (startSym ag)]
+              (s1 ++ [NTS lhs] ++ s2)`
+	    by METIS_TAC [RTC_NRC] THEN
+	    `?n.NRC (rderives ag) n 
+              [NTS (startSym ag)]
+              (s1 ++ [NTS lhs'] ++ s2)`
+	    by METIS_TAC [RTC_NRC] THEN
+	    IMP_RES_TAC lemma THEN
+	    `(s=s') /\ (s=s'') /\ (s=s''')`
+	    by METIS_TAC [transOutEq] THEN
+	    SRW_TAC [][] THEN
+	    Cases_on `lhs=startSym ag` THEN
+	    SRW_TAC [][]
+            THENL[
+		  `rhs=[NTS (startSym g);TS eof]`
+		      by METIS_TAC [auggrStartRule] THEN
+		  METIS_TAC [auggrEofInRhs,APPEND,APPEND_NIL],
+		  
+		  `¬(s2=[])` by METIS_TAC [lastEof,MEM,MEM_APPEND] THEN
+		  Cases_on `s2` THEN FULL_SIMP_TAC (srw_ss()) [] THEN
+		  SRW_TAC [][] THEN
+		  `h IN (followSet ag (NTS lhs))` by METIS_TAC [followSetMem, APPEND, APPEND_ASSOC, APPEND_NIL, rtcRdImpDg, isTmnlSym_def] THEN
+		  `h IN (followSet ag (NTS lhs'))` by METIS_TAC [followSetMem, APPEND, APPEND_ASSOC, APPEND_NIL, rtcRdImpDg, isTmnlSym_def] THEN
+		  IMP_RES_TAC ruleRhsExistsImpTrans THEN
+		  `∃s'. trans ag (s,rhs) = SOME s'` by METIS_TAC [] THEN
+		  `trans ag (initItems ag (rules ag),s1++rhs) = SOME s'`
+		  by METIS_TAC [transSeq,initItems_def] THEN
+		  `validItem ag (s1++rhs) (item lhs' (rhs,[]))`
+		  by (SRW_TAC [][validItem_def] THEN
+		      Q.EXISTS_TAC `h::t` THEN
+		      SRW_TAC [][] THEN
+		      METIS_TAC [EVERY_DEF,rdres1,rderives_append]) THEN
+		  `validItem ag (s1++rhs) (item lhs (rhs,[]))`
+		  by (SRW_TAC [][validItem_def] THEN
+		      Q.EXISTS_TAC `h::t` THEN
+		      SRW_TAC [][] THEN
+		      METIS_TAC [EVERY_DEF,rdres1,rderives_append]) THEN
+		  METIS_TAC [transImpValidItem,completeItem_def,itemLhs_def,slrCompItemsEq]
+		  ],
+
+
+	    FULL_SIMP_TAC (srw_ss()) [rsf_def] THEN
+	    Cases_on `lhs=startSym ag` THEN
+	    SRW_TAC [][]
+	    THENL[
+		  `rhs=[NTS (startSym g);TS eof]` by METIS_TAC [auggrStartRule] THEN
+		  SRW_TAC [][] THEN
+		  `(p ++ [NTS (startSym g); TS eof] = 
+                      (p++[NTS (startSym g)])++[TS eof]++[])`
+		      by METIS_TAC [APPEND,APPEND_ASSOC,APPEND_NIL] THEN
+		  `(p++[NTS (startSym g)]=[NTS (startSym g)]) /\ (lhs'=startSym ag)`
+		      by METIS_TAC [auggrEofInRhs,APPEND_ASSOC] THEN		  
+		  Cases_on `p` THEN FULL_SIMP_TAC (srw_ss()) [],
+
+		  `¬(s2=[])` by METIS_TAC [lastEof,MEM,MEM_APPEND] THEN
+		  Cases_on `s2` THEN FULL_SIMP_TAC (srw_ss()) [] THEN
+		  SRW_TAC [][] THEN
+		  `h IN (followSet ag (NTS lhs))` by METIS_TAC [followSetMem, APPEND, APPEND_ASSOC, APPEND_NIL, rtcRdImpDg, isTmnlSym_def] THEN
+		  `h IN (followSet ag (NTS lhs'))` by METIS_TAC [followSetMem, APPEND, APPEND_ASSOC, APPEND_NIL, rtcRdImpDg, isTmnlSym_def] THEN
+		  Cases_on `p=[]` THEN SRW_TAC [][]
+                  THENL[
+			FULL_SIMP_TAC (srw_ss()) []  THEN
+			`?n.NRC (rderives ag) n [NTS (startSym ag)]
+              		  (s1' ++ [NTS lhs] ++ h::t)`
+			    by METIS_TAC [RTC_NRC] THEN
+			IMP_RES_TAC lemma THEN
+			IMP_RES_TAC ruleRhsExistsImpTrans THEN
+			`∃s''. trans ag (s',rhs) = SOME s''` by METIS_TAC [] THEN
+			`trans ag (initItems ag (rules ag),s1'++rhs) = SOME s''`
+			    by METIS_TAC [transSeq,initItems_def] THEN
+			`validItem ag (s1'++rhs) (item lhs (rhs,[]))`
+			    by (SRW_TAC [][validItem_def] THEN
+				Q.EXISTS_TAC `h::t` THEN
+				SRW_TAC [][] THEN
+				METIS_TAC [EVERY_DEF,rdres1,rderives_append]) THEN
+			`validItem ag (s1'++rhs) (item lhs' (rhs,[]))`
+			    by (SRW_TAC [][validItem_def] THEN
+				Q.EXISTS_TAC `h::t` THEN
+				SRW_TAC [][] THEN
+				METIS_TAC [EVERY_DEF,rdres1,rderives_append]) THEN
+			METIS_TAC [transImpValidItem,completeItem_def,itemLhs_def,slrCompItemsEq],
+
+			`?n.NRC (rderives ag) n [NTS (startSym ag)]
+              		  (s1' ++ p++ [NTS lhs] ++ h::t)`
+			    by METIS_TAC [RTC_NRC] THEN
+			IMP_RES_TAC lemma THEN
+			IMP_RES_TAC ruleRhsExistsImpTrans THEN
+			`∃s''. trans ag (s',rhs) = SOME s''` by METIS_TAC [] THEN
+			`trans ag (initItems ag (rules ag),s1'++p++rhs) = SOME s''`
+			    by METIS_TAC [transSeq,initItems_def] THEN
+			`validItem ag (s1'++p++rhs) (item lhs (rhs,[]))`
+			    by (SRW_TAC [][validItem_def] THEN
+				Q.EXISTS_TAC `h::t` THEN
+				SRW_TAC [][] THEN
+				METIS_TAC [EVERY_DEF,rdres1,rderives_append]) THEN
+			`validItem ag (s1'++p++rhs) (item lhs' (p++rhs,[]))`
+			    by (SRW_TAC [][validItem_def] THEN
+				Q.EXISTS_TAC `h::t` THEN
+				SRW_TAC [][] THEN
+				METIS_TAC [EVERY_DEF,rdres1,rderives_append,APPEND_ASSOC]) THEN
+			`?e t.p=e::t` by METIS_TAC [list_nchotomy] THEN
+			SRW_TAC [][] THEN			
+			`(item lhs' (e::t' ++ rhs,[])=(item lhs (rhs,[])))` 
+				    by METIS_TAC [transImpValidItem,completeItem_def,itemLhs_def,slrCompItemsEq] THEN
+			FULL_SIMP_TAC (srw_ss()) [] THEN
+			METIS_TAC [APPEND,APPEND_11,NOT_CONS_NIL]
+			]
+		  ],
+		  
+	    SRW_TAC [][] THEN
+	    FULL_SIMP_TAC (srw_ss()) []  THEN
+	    FULL_SIMP_TAC (srw_ss()) [rsf_def] THEN
+	    Cases_on `lhs=startSym ag` THEN
+	    SRW_TAC [][]
+            THENL[
+		  `p++rhs'=[NTS (startSym g);TS eof]` by METIS_TAC [auggrStartRule] THEN
+		  Cases_on `p` THEN Cases_on `rhs'` THEN SRW_TAC [][] THEN
+		  FULL_SIMP_TAC (srw_ss()) [] THEN
+		  SRW_TAC [][] 
+		  THENL[
+			      METIS_TAC [auggrEofInRhs,APPEND,APPEND_NIL],
+
+			      `(s1=[]) /\ (s2=[])`
+				  by METIS_TAC [auggrRtcRderivesPfxSfxNil,MEM,MEM_APPEND] THEN
+			      SRW_TAC [][] THEN
+			      FULL_SIMP_TAC (srw_ss()) [] THEN
+			      Cases_on `lhs'=startSym ag` THEN
+			      SRW_TAC [][] 
+			      THENL[
+				    `[NTS (startSym g); TS eof; NTS (startSym ag)] = [NTS (startSym g); TS eof]++ [NTS (startSym ag)]++[]`
+					by METIS_TAC [APPEND,APPEND_NIL] THEN
+				    METIS_TAC [auggrRtcRderivesPfxSfxNil,MEM,MEM_APPEND],
+			      
+				    `[NTS (startSym g); TS eof; NTS lhs']=[NTS (startSym g); TS eof]++ [NTS lhs']`
+					by METIS_TAC [APPEND] THEN
+				    METIS_TAC [APPEND_NIL,lastEof,MEM,MEM_APPEND]
+				    ],
+
+			      Cases_on `t'` THEN Cases_on `t` THEN
+			      FULL_SIMP_TAC (srw_ss()) [] THEN
+			      SRW_TAC [][] THEN
+			      METIS_TAC [APPEND_NIL,NOT_CONS_NIL,auggrEofInRhs]				    
+			      ],
+		  
+		  `¬(s2=[])` by METIS_TAC [lastEof,MEM,MEM_APPEND] THEN
+		  Cases_on `s2` THEN FULL_SIMP_TAC (srw_ss()) [] THEN
+		  SRW_TAC [][] THEN
+		  `h IN (followSet ag (NTS lhs))` by METIS_TAC [followSetMem, APPEND, APPEND_ASSOC, APPEND_NIL, rtcRdImpDg, isTmnlSym_def] THEN
+		  `h IN (followSet ag (NTS lhs'))` by METIS_TAC [followSetMem, APPEND, APPEND_ASSOC, APPEND_NIL, rtcRdImpDg, isTmnlSym_def] THEN
+		  `?n.NRC (rderives ag) n [NTS (startSym ag)]
+              		(s1 ++ p++ [NTS lhs'] ++ h::t)`
+		      by METIS_TAC [RTC_NRC] THEN
+		  IMP_RES_TAC lemma THEN
+		  IMP_RES_TAC ruleRhsExistsImpTrans THEN
+		  `∃s''. trans ag (s',rhs') = SOME s''` by METIS_TAC [] THEN
+		  `trans ag (initItems ag (rules ag),s1++p++rhs') = SOME s''`
+		      by METIS_TAC [transSeq,initItems_def] THEN
+		  `validItem ag (s1++p++rhs') (item lhs' (rhs',[]))`
+		      by (SRW_TAC [][validItem_def] THEN
+			  Q.EXISTS_TAC `h::t` THEN
+			  SRW_TAC [][] THEN
+			  METIS_TAC [EVERY_DEF,rdres1,rderives_append]) THEN
+		  `validItem ag (s1++p++rhs') (item lhs (p++rhs',[]))`
+		      by (SRW_TAC [][validItem_def] THEN
+			  Q.EXISTS_TAC `h::t` THEN
+			  SRW_TAC [][] THEN
+			  METIS_TAC [EVERY_DEF,rdres1,rderives_append,APPEND_ASSOC]) THEN
+		  Cases_on `p=[]` THEN SRW_TAC [][]
+                   THENL[
+			      FULL_SIMP_TAC (srw_ss()) [] THEN
+			      METIS_TAC [transImpValidItem,completeItem_def,itemLhs_def,slrCompItemsEq],
+			      
+			      `?e t.p=e::t` by METIS_TAC [list_nchotomy] THEN
+			      SRW_TAC [][] THEN			
+			      `(item lhs (e::t' ++ rhs',[])=(item lhs' (rhs',[])))` 
+				  by METIS_TAC [transImpValidItem,completeItem_def,itemLhs_def,slrCompItemsEq] THEN
+			      FULL_SIMP_TAC (srw_ss()) [] THEN
+			      METIS_TAC [APPEND,APPEND_11,NOT_CONS_NIL]
+			      ]		  
+			]
+		  ],
+      
+      FULL_SIMP_TAC (srw_ss()) [] THEN
+      SRW_TAC [][] THEN
+      METIS_TAC [slrConf1,EVERY_APPEND],
+
+      FULL_SIMP_TAC (srw_ss()) [] THEN
+      SRW_TAC [][] THEN
+      METIS_TAC [slrConf1,EVERY_APPEND]
+      ])       
+		       
+		       
+
+
+val ambThm0 = store_thm
+("ambThm0",
+ ``(auggr g st eof = SOME ag) ==>
+ (!nt.nt ∈ nonTerminals ag ==> gaw ag nt) ==> 
+ (slr ag = SOME m) ==>
+  rtc2list (rderives ag) dl ==>
+ rtc2list (rderives ag) dl' ==>
+(HD dl = [NTS (startSym ag)]) ==>
+ (HD dl = HD dl') ==>
+ (LAST dl = LAST dl') ==>
+ EVERY isTmnlSym (LAST dl) ==>
+ (dl=dl')``,
+SRW_TAC [][] THEN
+SPOSE_NOT_THEN ASSUME_TAC THEN
+IMP_RES_TAC listDiffSfxSame
+THENL[
+      SRW_TAC [] [] THEN
+      Cases_on `pfx` THEN FULL_SIMP_TAC (srw_ss()) [] THEN
+      Cases_on `dl'` THEN FULL_SIMP_TAC (srw_ss()) [] THEN
+      SRW_TAC [][] THEN
+      FULL_SIMP_TAC (srw_ss()) [rtc2list_def] THEN
+      `rsf ag [NTS (startSym ag)]` by METIS_TAC [rsf_def,RTC_RULES] THEN
+      `TL ([NTS (startSym ag)]::
+                 (t ++ [NTS (startSym ag)]::t')) 
+          = (t ++ [NTS (startSym ag)]::t')` by SRW_TAC [][] THEN
+      IMP_RES_TAC rtc2listSt THEN
+      METIS_TAC [MEM,MEM_APPEND,APPEND,HD],
+
+      SRW_TAC [] [] THEN
+      Cases_on `pfx` THEN FULL_SIMP_TAC (srw_ss()) [] THEN
+      Cases_on `dl` THEN FULL_SIMP_TAC (srw_ss()) [] THEN
+      SRW_TAC [][] THEN
+      FULL_SIMP_TAC (srw_ss()) [rtc2list_def] THEN
+      `rsf ag [NTS (startSym ag)]` by METIS_TAC [rsf_def,RTC_RULES] THEN
+      `TL ([NTS (startSym ag)]::
+                 (t ++ [NTS (startSym ag)]::t')) 
+          = (t ++ [NTS (startSym ag)]::t')` by SRW_TAC [][] THEN
+      IMP_RES_TAC rtc2listSt THEN
+      METIS_TAC [MEM,MEM_APPEND,APPEND,HD],
+
+      SRW_TAC [][] THEN
+      FULL_SIMP_TAC (srw_ss()) [] THEN
+      Cases_on `pfx=[]` THEN SRW_TAC [][] THEN
+      FULL_SIMP_TAC (srw_ss()) [] THEN
+      Cases_on `pfx'=[]` THEN FULL_SIMP_TAC (srw_ss()) [] THEN
+      SRW_TAC [][] THEN
+      FULL_SIMP_TAC (srw_ss()) [] THEN
+      `¬(pfx'++[h']++sfx = [])`by SRW_TAC [][] THEN
+      `(pfx'++[h']++sfx = (HD (pfx'++[h']++sfx))::
+                           TL (pfx'++[h']++sfx))`
+	  by METIS_TAC [listHdTl,APPEND] THEN
+      Q.ABBREV_TAC `h = HD (pfx'++[h']++sfx)` THEN
+      Q.ABBREV_TAC `tl = TL (pfx'++[h']++sfx)` THEN
+      Q.ABBREV_TAC `ls = LAST (pfx'++[h']++sfx)` 
+      THENL[
+	    `rsf ag h` by METIS_TAC [rsf_def,RTC_RULES] THEN
+	    `∀e.MEM e tl ==> rsf ag e` 
+		by METIS_TAC [rsfDistribRtc2List] THEN
+	    Cases_on `sfx` THEN FULL_SIMP_TAC (srw_ss()) [] 
+           THENL[
+		 METIS_TAC [last_append,APPEND,NOT_CONS_NIL,LAST_CONS],
+	   
+		 `rderives ag h' h'' ` by METIS_TAC [rtc2listRd,APPEND,APPEND_ASSOC] THEN
+		 FULL_SIMP_TAC (srw_ss()) [rderives_def] THEN
+		 SRW_TAC [][] THEN
+		 FULL_SIMP_TAC (srw_ss()) [lreseq] THEN
+		 SRW_TAC [][] THEN
+		 FULL_SIMP_TAC (srw_ss()) [] THEN
+		 `rhs=[NTS (startSym g);TS eof]` by METIS_TAC [auggrStartRule] THEN
+		 SRW_TAC [][] 
+                 THENL[
+		       Cases_on `s1'` THEN FULL_SIMP_TAC (srw_ss()) [] THEN
+		       Cases_on `t'` THEN FULL_SIMP_TAC (srw_ss()) [] THEN
+		       SRW_TAC [][] 
+		       THENL[
+		       Cases_on `rhs'` THEN SRW_TAC [][] THEN
+		       FULL_SIMP_TAC (srw_ss()) [] THEN
+		       SRW_TAC [][] THEN
+		       Cases_on `pfx'` THEN FULL_SIMP_TAC (srw_ss()) [] THEN
+		       SRW_TAC [][] 
+               	       THENL[
+			     `rderives ag [NTS (startSym g); NTS lhs'; TS eof]
+		               [NTS (startSym g); TS eof] ` 
+				 by METIS_TAC [rtc2listRd,APPEND,APPEND_ASSOC] THEN
+			     FULL_SIMP_TAC (srw_ss()) [rderives_def] THEN
+			     SRW_TAC [][] THEN
+			     Cases_on `s1` THEN FULL_SIMP_TAC (srw_ss()) [] THEN
+			     SRW_TAC [][] THEN
+			     FULL_SIMP_TAC (srw_ss()) [isTmnlSym_def] THEN
+			     Cases_on `t''` THEN FULL_SIMP_TAC (srw_ss()) [] THEN
+			     SRW_TAC [][] THEN
+			     Cases_on `rhs` THEN FULL_SIMP_TAC (srw_ss()) []THEN
+			     SRW_TAC [][] THEN
+			     `RTC (rderives ag) [NTS (startSym ag)] [NTS (startSym g); NTS lhs; TS eof]`
+				 by METIS_TAC [rsf_def,MEM,MEM_APPEND,APPEND] THEN
+			     `?n.NRC (rderives ag) n [NTS (startSym ag)]
+		                 ([NTS (startSym g)]++[NTS lhs]++[TS eof])` 
+				 by METIS_TAC [RTC_NRC,APPEND,rdres1,RTC_RULES,APPEND_NIL] THEN
+			     `∃s.(trans ag (initItems ag (rules ag),[NTS (startSym g)]) 
+				  = SOME s) ∧
+		                   MEM (item lhs ([],[])) s` by METIS_TAC [lemma] THEN
+			     `validItem ag [NTS (startSym g)] 
+		                   (item (startSym ag) ([NTS (startSym g)],[TS eof]))` 
+				 by (SRW_TAC [] [validItem_def] THEN
+				     MAP_EVERY Q.EXISTS_TAC [`[]`,`[]`] THEN
+				     SRW_TAC [] [RTC_RULES]  THEN
+				     METIS_TAC [rdres1]) THEN
+			     `MEM (item (startSym ag) ([NTS (startSym g)],[TS eof]))
+		              s` by METIS_TAC [transImpValidItem] THEN
+			     `(TS eof) IN (followSet ag (NTS lhs))` by METIS_TAC [followSetMem, APPEND, APPEND_ASSOC, APPEND_NIL, rtcRdImpDg, isTmnlSym_def] THEN	   
+			     METIS_TAC [slrNotValid,isTmnlSym_def,sgoto_exp],
+			     
+			     METIS_TAC [auggrEofInRhs,APPEND,NOT_CONS_NIL]
+			     ],
+	   
+
+		       (*cases on t'*)
+		       SRW_TAC [][] THEN
+		       FULL_SIMP_TAC (srw_ss()) [] THEN
+		       `RTC (rderives ag) [NTS (startSym ag)] [NTS (startSym g);TS eof;NTS lhs']`
+			   by METIS_TAC [rsf_def,MEM,MEM_APPEND,APPEND] THEN
+		       `[NTS (startSym g); TS eof; NTS lhs'] =
+         		 [NTS (startSym g); TS eof] ++[NTS lhs']++[]`
+			   by METIS_TAC [APPEND,APPEND_NIL] THEN
+		       Cases_on `lhs'=startSym ag` 
+			THENL[
+			      METIS_TAC [APPEND,auggrRtcRderivesPfxSfxNil,NOT_CONS_NIL],
+			      
+			      METIS_TAC [MEM,MEM_APPEND,lastEof]
+			      ]
+		       ],
+
+		       
+		       Cases_on `s2'` THEN FULL_SIMP_TAC (srw_ss()) [] THEN
+		       Cases_on `t'` THEN FULL_SIMP_TAC (srw_ss()) [] THEN
+		       SRW_TAC [][] 
+		       THENL[
+                       Cases_on `s1'` THEN
+		       Cases_on `rhs'` THEN SRW_TAC [][] THEN
+		       FULL_SIMP_TAC (srw_ss()) [] THEN
+		       SRW_TAC [][] THEN
+		       Cases_on `pfx'` THEN FULL_SIMP_TAC (srw_ss()) [] THEN
+		       SRW_TAC [][] 
+               	       THENL[
+			     Cases_on `t'` THEN FULL_SIMP_TAC (srw_ss()) [] THEN
+			     SRW_TAC [][] THEN
+			     `rsf ag [NTS lhs'; TS eof]`
+				 by METIS_TAC [MEM,MEM_APPEND] THEN
+			     FULL_SIMP_TAC (srw_ss()) [rsf_def] THEN
+			     `?n.NRC (rderives ag) n [NTS (startSym ag)]
+		                 ([]++[NTS lhs']++[TS eof])` 
+				 by METIS_TAC [RTC_NRC,APPEND,rdres1,RTC_RULES,APPEND_NIL] THEN
+			     `∃s.(trans ag (initItems ag (rules ag),[]) 
+				  = SOME s) ∧
+		                   MEM (item lhs' ([],[NTS (startSym g)])) s` by METIS_TAC [lemma] THEN
+			     FULL_SIMP_TAC (srw_ss()) [trans_def] THEN
+			     SRW_TAC [][] THEN
+			     `MEM (rule (startSym ag) [NTS (startSym g); TS eof])
+				   (rules ag)` by METIS_TAC [auggrNewRuleMem] THEN
+			     `MEM (item (startSym ag) ([],[NTS (startSym g);TS eof]))
+				   (initItems ag (rules ag))` by METIS_TAC [memInitProds] THEN
+			     `(TS eof) IN (followSet ag (NTS lhs'))`
+				 by METIS_TAC [followSetMem, APPEND, APPEND_ASSOC, APPEND_NIL, rtcRdImpDg, isTmnlSym_def] THEN	   
+			     `?s.(trans ag (initItems ag (rules ag),[NTS (startSym g)]) = SOME s)
+                               /\ MEM (item lhs' ([NTS (startSym g)],[])) s 
+                               /\ MEM (item (startSym ag) ([NTS (startSym g)],[TS eof])) s`
+				 by (SRW_TAC [][] THEN
+				     FULL_SIMP_TAC (srw_ss()) [trans_def] THEN
+				     `MEM (item lhs' ([NTS (startSym g)],[]))
+                                 (moveDot (initItems ag (rules ag)) (NTS (startSym g)))`
+					 by METIS_TAC [APPEND,mdMemExists] THEN
+				     `MEM (item (startSym ag) ([NTS (startSym g)],[TS eof]))
+                                 (moveDot (initItems ag (rules ag)) (NTS (startSym g)))`
+					 by METIS_TAC [APPEND,mdMemExists] THEN
+				     Cases_on `moveDot (initItems ag (rules ag)) (NTS (startSym g))` THEN
+				     FULL_SIMP_TAC (srw_ss()) [] THEN
+				     METIS_TAC [iclosure_mem,MEM]) THEN
+			     METIS_TAC [slrNotValid,isTmnlSym_def,sgoto_exp],
+
+			     Cases_on `t'` THEN FULL_SIMP_TAC (srw_ss()) [] THEN
+			     SRW_TAC [][] THEN
+			     `RTC (rderives ag) [NTS (startSym ag)] [NTS (startSym g); NTS lhs'; TS eof]`
+				 by METIS_TAC [rsf_def,MEM,MEM_APPEND,APPEND] THEN
+			     `?n.NRC (rderives ag) n [NTS (startSym ag)]
+		                 ([NTS (startSym g)]++[NTS lhs']++[TS eof])` 
+				 by METIS_TAC [RTC_NRC,APPEND,rdres1,RTC_RULES,APPEND_NIL] THEN
+			     `∃s.(trans ag (initItems ag (rules ag),[NTS (startSym g)]) 
+				  = SOME s) ∧
+		                   MEM (item lhs' ([],[])) s` by METIS_TAC [lemma] THEN
+			     `validItem ag [NTS (startSym g)] 
+		                   (item (startSym ag) ([NTS (startSym g)],[TS eof]))` 
+				 by (SRW_TAC [] [validItem_def] THEN
+				     MAP_EVERY Q.EXISTS_TAC [`[]`,`[]`] THEN
+				     SRW_TAC [] [RTC_RULES]  THEN
+				     METIS_TAC [rdres1]) THEN
+			     `MEM (item (startSym ag) ([NTS (startSym g)],[TS eof]))
+		              s` by METIS_TAC [transImpValidItem] THEN
+			     `(TS eof) IN (followSet ag (NTS lhs'))` by METIS_TAC [followSetMem, APPEND, APPEND_ASSOC, APPEND_NIL, rtcRdImpDg, isTmnlSym_def] THEN	   
+			     METIS_TAC [slrNotValid,isTmnlSym_def,sgoto_exp],
+			     
+			     Cases_on `t'` THEN SRW_TAC [][] THEN
+			     FULL_SIMP_TAC (srw_ss()) []
+			     ],
+	   
+		       
+		       (*cases on s2'*)
+		       Cases_on `s1'` THEN 
+		       Cases_on `rhs'` THEN
+		       FULL_SIMP_TAC (srw_ss()) [] THEN
+		       SRW_TAC [] [] THEN
+		       FULL_SIMP_TAC (srw_ss()) [isTmnlSym_def] THEN
+		       Cases_on `t'` THEN FULL_SIMP_TAC (srw_ss()) []
+		       ],
+
+		       Cases_on `s1'` THEN
+		       Cases_on `rhs'` THEN
+		       Cases_on `s2'` THEN
+		       SRW_TAC [][] THEN
+		       FULL_SIMP_TAC (srw_ss()) [] THEN
+		       SRW_TAC [][] THEN
+		       FULL_SIMP_TAC (srw_ss()) [isTmnlSym_def]
+                       THENL[
+			     METIS_TAC [auggrEofInRhs,APPEND,APPEND_NIL],
+
+			     SRW_TAC [][] THEN
+			     Cases_on `t'` THEN FULL_SIMP_TAC (srw_ss()) [] THEN
+			     SRW_TAC [][] THEN
+			     Cases_on `pfx'` THEN SRW_TAC [][] THEN
+			     FULL_SIMP_TAC (srw_ss()) [] THEN
+			     `rderives ag [NTS lhs'; TS eof] [NTS (startSym g); TS eof]`
+			     by METIS_TAC [rtc2listRd,APPEND,APPEND_ASSOC] THEN
+			     `rsf ag [NTS lhs'; TS eof]` by METIS_TAC [MEM,MEM_APPEND] THEN
+			     FULL_SIMP_TAC (srw_ss()) [rsf_def] THEN
+			     `?n.NRC (rderives ag) n [NTS (startSym ag)]
+                		       [NTS lhs'; TS eof]` by METIS_TAC [RTC_NRC] THEN
+			     `MEM (item lhs' ([],[NTS (startSym g)])) (initItems ag (rules ag))`
+			     by METIS_TAC [initItemsHdNt,APPEND] THEN
+			     `MEM (item (startSym ag) ([],[NTS (startSym g);TS eof]))
+				       (initItems ag (rules ag))` 
+				 by METIS_TAC [memInitProds] THEN
+			     `?s.(trans ag (initItems ag (rules ag),[NTS (startSym g)]) = SOME s)
+                               /\ MEM (item (startSym ag)
+					     ([NTS (startSym g)], [TS eof])) s
+                               /\ MEM (item lhs' ([NTS (startSym g)],[])) s`
+			     by (SRW_TAC [] [trans_def] THEN
+				 Cases_on `moveDot (initItems ag (rules ag)) (NTS (startSym g))` THEN
+				 SRW_TAC [][] THEN
+				 METIS_TAC [mdMemExists,APPEND,MEM,iclosure_mem]) THEN
+			     `(TS eof) IN (followSet ag (NTS lhs'))` by METIS_TAC [followSetMem, APPEND, APPEND_ASSOC, APPEND_NIL, rtcRdImpDg, isTmnlSym_def] THEN			     
+			     METIS_TAC [slrNotValid,sgoto_exp,isTmnlSym_def],
+
+
+			     `rsf ag [NTS (startSym g); TS eof; NTS lhs']`
+			     by METIS_TAC [MEM,MEM_APPEND,APPEND] THEN
+			     `[NTS (startSym g); TS eof; NTS lhs']=[NTS (startSym g); TS eof] ++[NTS lhs']++[]`
+				 by METIS_TAC [APPEND,APPEND_NIL] THEN
+			     METIS_TAC [lastEof,MEM,MEM_APPEND,rsf_def],
+
+			     Cases_on `t'` THEN
+			     FULL_SIMP_TAC (srw_ss()) [] THEN
+			     SRW_TAC [][] THEN
+			     Cases_on `pfx'` THEN SRW_TAC [][] THEN
+			     FULL_SIMP_TAC (srw_ss()) [] THEN
+			     `rderives ag [NTS (startSym g); NTS lhs'; TS eof] [NTS (startSym g); TS eof]`
+			     by METIS_TAC [rtc2listRd,APPEND,APPEND_ASSOC] THEN
+			     `rsf ag [NTS (startSym g); NTS lhs'; TS eof]` by METIS_TAC [MEM,MEM_APPEND] THEN
+			     FULL_SIMP_TAC (srw_ss()) [rsf_def] THEN
+			     `?n.NRC (rderives ag) n [NTS (startSym ag)]
+                		       ([NTS (startSym g)]++[NTS lhs']++[TS eof])` by METIS_TAC [RTC_NRC,APPEND] THEN
+			     IMP_RES_TAC lemma THEN
+			     `MEM (item (startSym ag) ([],[NTS (startSym g);TS eof]))
+				       (initItems ag (rules ag))` 
+				 by METIS_TAC [memInitProds] THEN
+			     `validItem ag [NTS (startSym g)] (item (startSym ag) ([NTS (startSym g)],[TS eof]))`
+				 by (SRW_TAC [] [validItem_def] THEN
+				     MAP_EVERY Q.EXISTS_TAC [`[]`,`[]`] THEN
+				     SRW_TAC [][] THEN
+				     METIS_TAC [rdres1,rderives_append]) THEN
+			     `(TS eof) IN (followSet ag (NTS lhs'))` by METIS_TAC [followSetMem, APPEND, APPEND_ASSOC, APPEND_NIL, rtcRdImpDg, isTmnlSym_def] THEN			     
+			     METIS_TAC [slrNotValid,sgoto_exp,isTmnlSym_def,transImpValidItem],
+
+
+			     Cases_on `t'` THEN FULL_SIMP_TAC (srw_ss()) [] THEN
+			     SRW_TAC [][] THEN
+			     METIS_TAC [auggrEofInRhs,APPEND_NIL],
+
+			     Cases_on `t'` THEN FULL_SIMP_TAC (srw_ss()) []
+			     
+			     ]]],
+
+
+		 Cases_on `sfx=[]` THEN
+		 SRW_TAC [][] THEN
+		 FULL_SIMP_TAC (srw_ss()) [isTmnlSym_def] THEN
+		 `∃e t.sfx=e::t` by METIS_TAC [list_nchotomy] THEN
+		 SRW_TAC [][] THEN
+		 Cases_on `pfx` THEN SRW_TAC [][] THEN
+		 FULL_SIMP_TAC (srw_ss()) [] THEN
+		 `rsf ag [NTS (startSym ag)]` by METIS_TAC [rsf_def,RTC_RULES] THEN
+		 `rderives ag h e`by METIS_TAC [rtc2listRd,APPEND,APPEND_ASSOC] THEN
+		 FULL_SIMP_TAC (srw_ss()) [rderives_def,lreseq] THEN
+		 SRW_TAC [][] THEN
+		 `s1++rhs++s2=[NTS (startSym g);TS eof]`
+		 by METIS_TAC [auggrStartRule] THEN
+		 Cases_on `s1` THEN
+		 Cases_on `rhs` THEN
+		 Cases_on `s2` THEN
+		 FULL_SIMP_TAC (srw_ss()) [] THEN
+		 SRW_TAC [][] THEN
+		 FULL_SIMP_TAC (srw_ss()) [isTmnlSym_def]
+		 THENL[
+		       METIS_TAC [auggrEofInRhs,APPEND,APPEND_NIL],
+
+		       Cases_on `t''` THEN SRW_TAC [][] THEN
+		       FULL_SIMP_TAC (srw_ss()) [] THEN
+		       SRW_TAC [][] THEN
+		       IMP_RES_TAC rsfDistribRtc2List THEN
+		       `rsf ag [NTS lhs; TS eof]` by METIS_TAC [rsfDistribRtc2List,MEM,MEM_APPEND,APPEND] THEN
+		       FULL_SIMP_TAC (srw_ss()) [rsf_def] THEN
+		       `?n.NRC (rderives ag) n [NTS (startSym ag)]
+         		 ([]++[NTS lhs]++[TS eof])` 
+			   by METIS_TAC [RTC_NRC,APPEND,rdres1,RTC_RULES,APPEND_NIL] THEN
+		       `∃s.(trans ag (initItems ag (rules ag),[]) 
+				  = SOME s) ∧
+		                   MEM (item lhs ([],[NTS (startSym g)])) s` by METIS_TAC [lemma] THEN
+			     FULL_SIMP_TAC (srw_ss()) [trans_def] THEN
+			     SRW_TAC [][] THEN
+			     `MEM (rule (startSym ag) [NTS (startSym g); TS eof])
+				   (rules ag)` by METIS_TAC [auggrNewRuleMem] THEN
+			     `MEM (item (startSym ag) ([],[NTS (startSym g);TS eof]))
+				   (initItems ag (rules ag))` by METIS_TAC [memInitProds] THEN
+			     `(TS eof) IN (followSet ag (NTS lhs))`
+				 by METIS_TAC [followSetMem, APPEND, APPEND_ASSOC, APPEND_NIL, rtcRdImpDg, isTmnlSym_def] THEN	   
+ 			     `?s.(trans ag (initItems ag (rules ag),[NTS (startSym g)]) = SOME s)
+                               /\ MEM (item lhs ([NTS (startSym g)],[])) s 
+                               /\ MEM (item (startSym ag) ([NTS (startSym g)],[TS eof])) s`
+				 by (SRW_TAC [][] THEN
+				     FULL_SIMP_TAC (srw_ss()) [trans_def] THEN
+				     `MEM (item lhs ([NTS (startSym g)],[]))
+                                 (moveDot (initItems ag (rules ag)) (NTS (startSym g)))`
+					 by METIS_TAC [APPEND,mdMemExists] THEN
+				     `MEM (item (startSym ag) ([NTS (startSym g)],[TS eof]))
+                                 (moveDot (initItems ag (rules ag)) (NTS (startSym g)))`
+					 by METIS_TAC [APPEND,mdMemExists] THEN
+				     Cases_on `moveDot (initItems ag (rules ag)) (NTS (startSym g))` THEN
+				     FULL_SIMP_TAC (srw_ss()) [] THEN
+				     METIS_TAC [iclosure_mem,MEM]) THEN
+			     METIS_TAC [slrNotValid,isTmnlSym_def,sgoto_exp],
+
+
+		       IMP_RES_TAC rsfDistribRtc2List THEN
+		       `rsf ag [NTS (startSym g); TS eof; NTS lhs]`
+			   by METIS_TAC [APPEND,MEM,MEM_APPEND] THEN
+		       FULL_SIMP_TAC (srw_ss()) [rsf_def] THEN
+		       Cases_on `lhs=startSym ag`
+		       THENL[
+			     METIS_TAC [auggrStartRule,APPEND,NOT_CONS_NIL],
+
+			     `[NTS (startSym g); TS eof; NTS lhs]=
+                              [NTS (startSym g); TS eof]++[NTS lhs]++[]`
+				 by METIS_TAC [APPEND,APPEND_ASSOC,APPEND_NIL] THEN
+			     METIS_TAC [MEM,MEM_APPEND,lastEof]
+			     ],
+
+
+
+		       Cases_on `t''` THEN SRW_TAC [][] THEN
+		       FULL_SIMP_TAC (srw_ss()) [] THEN	
+		       SRW_TAC [][] THEN
+		       IMP_RES_TAC rsfDistribRtc2List THEN
+		       `rsf ag [NTS (startSym g); NTS lhs; TS eof]`
+			   by METIS_TAC [APPEND,MEM,MEM_APPEND] THEN
+		       FULL_SIMP_TAC (srw_ss()) [rsf_def] THEN
+		       `?n.NRC (rderives ag) n [NTS (startSym ag)]
+		                 ([NTS (startSym g)]++[NTS lhs]++[TS eof])` 
+				 by METIS_TAC [RTC_NRC,APPEND,rdres1,RTC_RULES,APPEND_NIL] THEN
+			     `∃s.(trans ag (initItems ag (rules ag),[NTS (startSym g)]) 
+				  = SOME s) ∧
+		                   MEM (item lhs ([],[])) s` by METIS_TAC [lemma] THEN
+			     `validItem ag [NTS (startSym g)] 
+		                   (item (startSym ag) ([NTS (startSym g)],[TS eof]))` 
+				 by (SRW_TAC [] [validItem_def] THEN
+				     MAP_EVERY Q.EXISTS_TAC [`[]`,`[]`] THEN
+				     SRW_TAC [] [RTC_RULES]  THEN
+				     METIS_TAC [rdres1]) THEN
+			     `MEM (item (startSym ag) ([NTS (startSym g)],[TS eof]))
+		              s` by METIS_TAC [transImpValidItem] THEN
+			     `(TS eof) IN (followSet ag (NTS lhs))` by METIS_TAC [followSetMem, APPEND, APPEND_ASSOC, APPEND_NIL, rtcRdImpDg, isTmnlSym_def] THEN	   
+			     METIS_TAC [slrNotValid,isTmnlSym_def,sgoto_exp],
+
+		       Cases_on `t''` THEN FULL_SIMP_TAC (srw_ss()) [] THEN
+		       SRW_TAC [][] THEN
+		       METIS_TAC [auggrEofInRhs,APPEND,NOT_CONS_NIL],
+
+		       Cases_on `t''` THEN FULL_SIMP_TAC (srw_ss()) []
+		       ],
+
+
+		 Cases_on `pfx` THEN 
+		 Cases_on `pfx'` THEN
+		 Cases_on `sfx` THEN
+		 FULL_SIMP_TAC (srw_ss()) [] THEN
+		 SRW_TAC [][] THEN
+		 FULL_SIMP_TAC (srw_ss()) [isNonTmnlSym_def]
+		 THENL[
+		       `LAST ([NTS (startSym ag)]::(t ++ [h])) = LAST [h]`
+		       by METIS_TAC [last_append,APPEND,APPEND_ASSOC,NOT_CONS_NIL] THEN
+		       `LAST (h''''::(t' ++ [h'])) = LAST [h']`
+			   by METIS_TAC [last_append,APPEND,APPEND_ASSOC,NOT_CONS_NIL] THEN
+		       FULL_SIMP_TAC (srw_ss()) [],
+
+		       `rderives ag h h'''''` 
+			   by METIS_TAC [rtc2listRd,APPEND,APPEND_ASSOC] THEN
+		       `rderives ag h' h'''''` 
+			   by METIS_TAC [rtc2listRd,APPEND,APPEND_ASSOC] THEN
+		       IMP_RES_TAC rsfDistribRtc2List THEN
+		       `rsf ag h` by METIS_TAC [APPEND,MEM_APPEND,MEM,rsf_def,RTC_RULES] THEN
+		       `rsf ag h'` by METIS_TAC [APPEND,MEM_APPEND,MEM,rsf_def,RTC_RULES] THEN
+		       FULL_SIMP_TAC (srw_ss()) [rderives_def] THEN
+		       SRW_TAC [] [] THEN
+		       UNABBREV_ALL_TAC  THEN
+		       FULL_SIMP_TAC (srw_ss()) [] THEN
+		       SRW_TAC [][] THEN
+		       METIS_TAC [slrConf,EVERY_APPEND]
+		       ]]])
+		       
+
+val ambThm = store_thm ("ambThm",
+``(auggr g st eof = SOME ag) ⇒
+       (∀nt. nt ∈ nonTerminals ag ⇒ gaw ag nt) ⇒
+       (slr ag = SOME m) ⇒
+       isUnambiguous0 ag``,
+SRW_TAC [] [isUnambiguous0,listderiv_def,language_def,
+	    EXTENSION] THEN
+METIS_TAC [ambThm0])
